src/PlutusIR/Semantics/Static/normaliser_STLC/STLC_named.v
@@ -309,3 +309,4 @@ Proof.
     || replace T' with (rename Y Y' T); eauto; rewrite <- rename_preserves_size; eauto
     ].
 Qed.
+
