src/PlutusIR/Semantics/Static/normaliser_STLC/gu_naive/SN_STLC_named2.v
@@ -1,4 +1,4 @@
-(* From mathcomp Require Import ssreflect ssrbool eqtype ssrnat.
+From mathcomp Require Import ssreflect ssrbool eqtype ssrnat.
 From Coq Require Import ssrfun.
 Require Import Coq.Strings.String.
 Require Import Coq.Lists.List.
@@ -15,7 +15,7 @@ Unset Strict Implicit.
 Unset Printing Implicit Defensive.
 From PlutusCert Require Import STLC_named STLC_named_typing ARS.
 From PlutusCert Require Import alpha alpha_rename rename util alpha_ctx_sub freshness alpha_freshness alpha_step step alpha_sub.
-From PlutusCert Require Import SN_STLC_named_naive.
+From PlutusCert Require Import SN_STLC_named_naive pre constructions.
 
 (* Define an infix operator for bind *)
 Infix ">>=" := bind (at level 50, left associativity).
@@ -37,6 +37,10 @@ with neutral_Ty : term -> Prop :=
       normal_Ty T2 ->
       neutral_Ty (tmapp T1 T2).
 
+(* induction principle for mutual induction*)
+Scheme normal_Ty_mut := Induction for normal_Ty Sort Prop
+with neutral_Ty_mut := Induction for neutral_Ty Sort Prop.
+
 Inductive step_d : term -> term -> Set :=
 | step_beta_d (x : string) (A : type) (s t : term) :
     normal_Ty s ->
@@ -50,121 +54,344 @@ Inductive step_d : term -> term -> Set :=
 | step_abs_d x A s1 s2 :
     step_d s1 s2 -> step_d (tmlam x A s1) (tmlam x A s2).
 
+Lemma in_ftv_existsb_true t s :
+  In s (ftv t) -> existsb (eqb s) (ftv t) = true.
+Proof.
+  intros Hin.
+  apply existsb_exists.
+  exists s.
+  split; auto.
+  apply eqb_eq. auto.
+Qed.
 
-Lemma GU_substituteTCA_substituteT A x t s : 
-    GU_vars (tmapp (tmlam x A s) t) -> substituteTCA x t s = substituteT x t s.
+Lemma not_in_ftv_existsb_false t s :
+  ~ In s (ftv t) <-> existsb (eqb s) (ftv t) = false.
+Proof.
+  split.
+  - intros H.
+    apply Bool.not_true_iff_false.
+    intros He. apply existsb_exists in He.
+    destruct He as [x [Hin Heqb] ].
+    apply eqb_eq in Heqb. subst.
+    contradiction.
+  - intros H.
+    intros Hcontra. apply in_ftv_existsb_true in Hcontra.
+    rewrite H in Hcontra. discriminate.
+Qed.
+
+
+(* We need to change this to: GU s and no binder in s is free in t. Isnt that simply NC?*)
+Lemma GU_substituteTCA_sub x t s : 
+    NC s ((x, t)::nil) -> substituteTCA x t s = sub x t s.
 Proof.
 intros.
 induction s; simpl.
-- admit.
-- assert (x =? s = false) by admit. (* GU *)
-  rewrite H0.
+- destr_eqb_eq x s.
+  + autorewrite with substituteTCA. rewrite String.eqb_refl. reflexivity.
+  + autorewrite with substituteTCA. rewrite <- String.eqb_neq in H0. rewrite H0. reflexivity.
+- assert (x =? s = false).
+  {
+    apply nc_ftv_env with (x := s) in H. 
+    - unfold ftv_keys_env in H. apply not_in_cons in H.  destruct H as [H _]. rewrite <- String.eqb_sym. 
+      rewrite <- String.eqb_neq in H. assumption.
+    - apply btv_lam.
+  }
   autorewrite with substituteTCA.
   rewrite H0.
-  assert (existsb (eqb s) (ftv t) = false) by admit. (* GU *)
+  assert (existsb (eqb s) (ftv t) = false).
+  {
+    apply nc_ftv_env with (x := s) in H. 
+    - unfold ftv_keys_env in H. apply not_in_cons in H.  destruct H as [_ H]. apply not_in_app in H as [H _].
+      apply not_in_ftv_existsb_false. assumption.
+    - apply btv_lam.
+  } 
   rewrite H1.
   f_equal.
   apply IHs.
-  inversion H; auto; subst.
-  constructor.
-  + inversion H4.
-    constructor. subst.
-    inversion H6. auto. (* notin btv extends to lambdabody *) admit.
-  + assumption.
-  + intros.
-    specialize (H_btv_btv_empty x0 H2). admit.
-  + intros.
-    (* x0 in btv (tmlam x A s0), so also in btv (tmlam x A (tmlam s t0 s0))*)
-    admit.
-  + intros.
-     (* we can use H_ftv_btv_empty, and deduce that s is not equal to any of the btv of t.*)
-Admitted.
+  eapply nc_lam. eauto.
+- autorewrite with substituteTCA. f_equal.
+  + eapply IHs1; eapply nc_app_l. eauto.
+  + eapply IHs2; eapply nc_app_r. eauto.
+Qed.
 
 (* If t has globally unique binders (and free variables to make it easier)
     then deterministic step and naive step coincide*)
 Lemma GU_step_d_implies_step_na t t' : 
-    GU_vars t -> step_d t t' -> step_naive t t'.
+    GU t -> step_d t t' -> step_naive t t'.
 Proof.
     intros HGU_vars H.
     induction H.
     - (* we can be sure that no binder in s appears in t by global uniqueness*)
-     assert (substituteTCA x t s = substituteT x t s) as Hsub.
-     { 
-        eapply GU_substituteTCA_substituteT.
-        eauto.
-      }
-     rewrite Hsub.
-     apply step_beta.
+      assert (substituteTCA x t s = sub x t s) as Hsub.
+      { 
+          eapply GU_substituteTCA_sub.
+          eapply gu_applam_to_nc. eauto.
+        }
+      rewrite Hsub.
+      apply step_beta.
     - apply step_appL. auto. inversion HGU_vars; auto.
     - apply step_appR. auto. inversion HGU_vars; auto.
     - apply step_abs. auto. inversion HGU_vars; auto.
 Qed.
 
-Lemma alpha_capms_to_naive X U T:
-  {T' & Alpha [] T T' * Alpha [] (substituteTCA X U T) (substituteT X U T')}.
+Lemma substituteTCA_vacuous X T s s' R : Alpha R s s' -> ~ In X (ftv s) -> Alpha R (substituteTCA X T s) s'.
 Proof.
-exists (to_unique_binders T).
-  split; try apply to_unique_binders_alpha.
-  induction T.
-  - admit.
-  - 
-Admitted.
+  intros Ha_s H.
+  generalize dependent s.
+  generalize dependent R.
+  induction s'; intros; simpl; 
+      inversion Ha_s; subst; 
+      autorewrite with substituteTCA.
+  - apply not_in_ftv_var in H. 
+    rewrite <- String.eqb_neq in H.
+    rewrite H. constructor. auto.
+  - destr_eqb_eq X x; auto.
+    destruct (existsb (eqb x) (ftv T)).
+    + apply ftv_lam_negative in H; auto.
+      remember (fresh2 [(x, tmvar x); (X, T)] s1) as Y'; simpl.
+      constructor.
+      apply IHs'; eauto.
+      * eapply alpha_trans_rename_left; eauto.
+      * apply ftv_not_in_rename; auto.
+        symmetry. 
+        eapply fresh2_over_key_sigma; intuition.
+    + constructor.
+      eapply IHs'; auto.
+      eapply ftv_lam_negative; eauto.
+  - constructor.
+    + eapply IHs'1; eauto. eapply not_ftv_app_not_left; eauto.
+    + eapply IHs'2; eauto. eapply not_ftv_app_not_right; eauto.
+Qed.
 
-Lemma alpha_rename_binder_substituteT {y : string } {s : term} s' x t t' ren:
-  Alpha ((x, y)::ren) s s' ->
-  Alpha ren t t' ->
-  Alpha ren (substituteT x t s) (substituteT y t' s').
+Lemma subs_preserves_alpha' X T i : forall s s' R1 R2 R,
+  R ⊢ (tmvar X) ~ (tmvar X) ->
+  R ⊢ T ~ T ->
+  αCtxTrans R1 R2 R ->
+  R1 ⊢ s ~ i ->
+  R2 ⊢ i ~ s' ->
+  R ⊢ substituteTCA X T s ~ substituteTCA X T s'.
 Proof.
-(* My assumption is that this is easier than for substituteTCA*)
-Admitted.
+  induction i as [xi | xi ? bi | i1 IHi1 i2 IHi2];
+  intros s s' R1 R2 R Ha_X Ha_T Htrans Hαs Hαs';
+  inversion Hαs as [xs ? ? Hαvs | xs ? ? bs ? ? Hαbs | s1 ? s2 ? ? Hαs1 Hαs2 ]; subst;
+  inversion Hαs' as [? xs' ? Hαvs' |? xs' ? ? bs' ? Hαbs' | ? s1' ? s2' ? Hαs1' Hαs2']; subst;
+  autorewrite with capms; simpl.
+  - (* Case: tmvar *)
+    repeat rewrite substituteTCA_equation_1.
+    assert (Hαv: AlphaVar R xs xs'). { eapply alpha_var_trans; eauto. }
+    destr_eqb_eq X xs.
+    + inversion Ha_X; subst.
+      apply (alphavar_unique_right H2) in Hαv. subst. rewrite String.eqb_refl. 
+      assumption.
+    + inversion Ha_X; subst.
+      remember (Hαv) as Hαv'. clear HeqHαv'.
+      apply (alphavar_unique_not_left H H3) in Hαv.
+      rewrite <- String.eqb_neq in Hαv.
+      rewrite Hαv. 
+      constructor.
+      auto.
+  - (* Case: tmlam *)
+    
+    (* remember (fresh2 _ bs) as b; rewrite cons_to_append in Heqb.
+    remember (fresh2 _ bs') as b'; rewrite cons_to_append in Heqb'. *)
+    (* idk, but it is true.*)
+    destr_eqb_eq xs X.
+    + rewrite substituteTCA_equation_2.
+      remember (fresh2 _ bs) as b; rewrite cons_to_append in Heqb.
+      rewrite String.eqb_refl.
+      eapply @alpha_sym with (ren := sym_alpha_ctx R); eauto with α_eq_db.
+      eapply substituteTCA_vacuous; eauto with α_eq_db.
+      eapply @alpha_preserves_no_ftv with (x := X) (s := tmlam X t bs).
+      * apply ftv_lam_no_binder.
+      * eauto with α_eq_db.
+      * inversion Ha_X; eauto.
+    + destr_eqb_eq xs' X.
+      * assert (substituteTCA X T (tmlam X t bs') = tmlam X t bs').
+        {
+          rewrite substituteTCA_equation_2.
+          rewrite String.eqb_refl.
+          reflexivity.
+        }
+        rewrite H0.
+        eapply substituteTCA_vacuous; eauto with α_eq_db.
+        eapply @alpha_preserves_no_ftv with (x := X) (s := tmlam X t bs').
+        -- apply ftv_lam_no_binder.
+        -- eauto with α_eq_db.
+        -- inversion Ha_X; eauto. eapply @alphavar_sym with (ren := R); eauto with α_eq_db.
+      * autorewrite with substituteTCA.
+        rewrite <- String.eqb_neq in H. rewrite String.eqb_sym in H. rewrite H.
+        rewrite <- String.eqb_neq in H0. rewrite String.eqb_sym in H0. rewrite H0.
+
+        destruct (existsb (eqb xs) (ftv T)) eqn:Hin; destruct (existsb (eqb xs') (ftv T)) eqn:Hin'.
+        -- simpl.
+           remember (fresh2 _ bs) as Y'.
+           remember (fresh2 _ bs') as Y''.
+           constructor.
+           eapply IHbi; eauto.
+           ++ eapply alpha_extend_fresh; auto.
+              ** eapply fresh2_over_key_sigma with (X := X) in HeqY'.
+                 intros Hcontra. apply ftv_var in Hcontra.  subst. contradiction.
+                 apply in_cons. apply in_eq.
+              ** eapply fresh2_over_key_sigma with (X := X) in HeqY''.
+                 intros Hcontra. apply ftv_var in Hcontra.  subst. contradiction.
+                 apply in_cons. apply in_eq.
+           ++ eapply alpha_extend_fresh; auto.
+              ** eapply fresh2_over_tv_value_sigma with (X := X) (s := T) in HeqY'.
+                 intros Hcontra. apply extend_ftv_to_tv in Hcontra. contradiction.
+                 apply in_cons. apply in_eq.
+              ** eapply fresh2_over_tv_value_sigma with (X := X) (s := T) in HeqY''.
+                 intros Hcontra. apply extend_ftv_to_tv in Hcontra. contradiction.
+                 apply in_cons. apply in_eq.
+           ++ constructor; eauto.
+           ++ eapply alpha_trans_rename_left; eauto.
+           ++ eapply alpha_trans_rename_right; eauto.
+        -- simpl.
+           remember (fresh2 _ bs) as Y'.
+           constructor.
+            eapply IHbi; eauto.
+            ++ eapply alpha_extend_fresh; auto.
+              ** eapply fresh2_over_key_sigma with (X := X) in HeqY'.
+                 intros Hcontra. apply ftv_var in Hcontra.  subst. contradiction.
+                 apply in_cons. apply in_eq.
+              ** intros Hcontra. apply ftv_var in Hcontra. subst.
+                 rewrite String.eqb_neq in H0. contradiction.
+            ++ eapply alpha_extend_fresh; auto.
+              ** eapply fresh2_over_tv_value_sigma with (X := X) (s := T) in HeqY'.
+                 intros Hcontra. apply extend_ftv_to_tv in Hcontra. contradiction.
+                 apply in_cons. apply in_eq.
+              ** eapply not_in_ftv_existsb_false. auto.
+            ++ eauto with α_eq_db.
+            ++ eapply alpha_trans_rename_left; eauto.
+        -- simpl.
+           remember (fresh2 _ _) as Y'.
+           constructor.
+           eapply IHbi; eauto. 
+           ++ eapply alpha_extend_fresh; auto.
+              ** intros Hcontra. apply ftv_var in Hcontra; subst.
+                  rewrite String.eqb_neq in H. contradiction.
+              **  
+                eapply fresh2_over_key_sigma with (X := X) in HeqY'.
+                 intros Hcontra. apply ftv_var in Hcontra.  subst. contradiction.
+                 apply in_cons. apply in_eq.
+
+           ++ eapply alpha_extend_fresh; auto.
+              eapply not_in_ftv_existsb_false. auto.
+              eapply fresh2_over_tv_value_sigma with (X := X) (s := T) in HeqY'.
+              intros Hcontra. apply extend_ftv_to_tv in Hcontra. contradiction.
+              apply in_cons. apply in_eq.
+           ++ constructor; eauto.
+           ++ eapply alpha_trans_rename_right; eauto.
+        -- constructor; eapply IHbi; eauto.
+           ++ apply alpha_extend_fresh; auto.
+              ** intros Hcontra. apply ftv_var in Hcontra; subst.
+                  rewrite String.eqb_neq in H. contradiction.
+              ** intros Hcontra. apply ftv_var in Hcontra; subst.
+                  rewrite String.eqb_neq in H0. contradiction.
+           ++ eapply alpha_extend_fresh; auto.
+              eapply not_in_ftv_existsb_false. auto.
+              eapply not_in_ftv_existsb_false. auto.
+           ++ eauto with α_eq_db.  
+  - autorewrite with substituteTCA.
+    constructor.
+    + eapply IHi1; eauto.
+    + eapply IHi2; eauto.
+Qed.
+
+Lemma substituteTCA_preserves_alpha s s' ren X U:
+  ren ⊢ (tmvar X) ~ (tmvar X) ->
+  (ren ⊢ U ~ U) ->
+  (ren ⊢ s ~ s') ->
+  Alpha ren (substituteTCA X U s) (substituteTCA X U s').
+Proof.
+  intros.
+  apply (@subs_preserves_alpha' X U s s s' (nil ++ ctx_id_left ren) ren ren); auto.
+  - apply id_left_trans; auto.
+  - apply alpha_extend_ids_right.
+    + apply ctx_id_left_is_id.
+    + apply alpha_refl. apply alpha_refl_nil.
+Qed.
+
+Lemma alpha_capms_to_naive X U T:
+  {T' & Alpha [] T T' * Alpha [] (substituteTCA X U T) (sub X U T') * NC T' ((X, U)::nil)}.
+Proof.
+  exists (to_GU' X U T).
+  split; [split|].
+  - apply to_GU'__alpha.
+  - eapply @alpha_trans with (t := substituteTCA X U (to_GU' X U T)).
+    constructor.
+    + eapply substituteTCA_preserves_alpha. eapply alpha_refl. constructor. eapply alpha_refl. constructor. apply to_GU'__alpha.
+    + erewrite GU_substituteTCA_sub.
+      * apply alpha_refl. constructor.
+      * apply to_GU'__NC.
+  - apply to_GU'__NC.
+Qed.
+
+Lemma alpha_preserves_normal_Ty__neutral_Ty s s' R :
+  R ⊢ s ~ s' -> ((normal_Ty s -> normal_Ty s') * (neutral_Ty s -> neutral_Ty s')).
+Proof.
+  intros Ha_s.
+  generalize dependent R.
+  generalize dependent s'.
+  induction s; intros s' R Ha_s; inversion Ha_s; subst.
+  - split; repeat constructor.
+  - edestruct IHs; eauto.
+    split.
+    + intros. constructor. eapply n. inversion H; subst. auto. inversion H0.
+    + intros. inversion H.
+  - edestruct IHs1; eauto.
+    edestruct IHs2; eauto.
+    split.
+    + intros. constructor. constructor.
+      * eapply n0. inversion H. inversion H0; subst. auto.
+      * inversion H; subst. inversion H0. auto.
+    + intros. inversion H; subst. constructor; eauto.
+Qed.
 
 Lemma alpha_preserves_normal_Ty s s' R :
   R ⊢ s ~ s' -> normal_Ty s -> normal_Ty s'.
 Proof.
-(* a normal_Ty cannot step.
-Suppose s' steps. Then by alpha_preserves_step we have that there is a corresponding step for s. Contradiction.
-*)
-Admitted.
+  intros Ha_s Hn.
+  edestruct (alpha_preserves_normal_Ty__neutral_Ty Ha_s) as [H _].
+  auto.
+Qed.
 
 (* Main lemma for going from using t alpha t' in SN t' to SN t*)
 Lemma step_d_preserves_alpha ren s t s' :
   Alpha ren s t -> step_d s s' -> {t' & (step_d t t') * (Alpha ren s' t')}%type.
 Proof.
-(* exists s'' s.t. step_gu_naive s s'' and s' ~ s''
-
-  We know s ~ t.
-
-  Supposinng we have step_gu_naive preserves alpha:
-  exists t'' s.t. step_gu_naive t t''   and s'' ~ t''
-
-  I think we then also have
-  exists t''' step_d t t'''. And since we also have s' ~ t'', the t' we are looking for is t''
-  
-  *)
   intros Halpha Hstep.
   generalize dependent t.
   generalize dependent ren.
   induction Hstep; intros ren t0 Halpha; inversion Halpha; subst.
   - inversion H2; subst.
     remember (alpha_capms_to_naive x t s).
-    destruct s1 as [s' [Halpha1 Halpha2] ].
+    destruct s1 as [s' [ [Halpha1 Halpha2] Halpha3] ].
     eexists.
     split.
     + apply step_beta_d; eapply alpha_preserves_normal_Ty; eauto.
-    + eapply @alpha_trans with (t := substituteT x t s').
+    + eapply @alpha_trans with (t := sub x t s').
       * apply id_left_trans.
       * change (ctx_id_left ren) with (nil ++ ctx_id_left ren).
         apply alpha_extend_ids_right.
         -- apply ctx_id_left_is_id.
         -- auto.
       * remember (alpha_capms_to_naive y t2 s0).
-        destruct s1 as [t' [Halpha1' Halpha2'] ].
+        destruct s1 as [t' [ [Halpha1' Halpha2'] Halpha3' ] ].
       
-        eapply @alpha_trans with (t := substituteT y t2 t').
+        eapply @alpha_trans with (t := sub y t2 t').
         -- apply id_right_trans.
-        -- eapply alpha_rename_binder_substituteT.
-           ++ (* follows directly from 3-fold transitivity*) admit.
-           ++ exact H4.
+        -- eapply alpha_rename_binder_stronger with (Rs := ((x, y)::ren)); eauto.
+           ++ eapply @alpha_trans with (t := s) (ren := ctx_id_left ((x, y)::ren)) (ren' := ((x, y)::ren)); eauto with α_eq_db.
+              ** apply id_left_trans.
+              ** apply alpha_extend_ids.
+                 --- apply ctx_id_left_is_id.
+                 --- eapply alpha_sym. constructor. eauto.
+              ** eapply @alpha_trans with (t := s0) (ren := ((x, y)::ren)) (ren' := ctx_id_right ((x, y)::ren)); eauto with α_eq_db.
+                  --- apply id_right_trans.
+                  --- apply alpha_extend_ids.
+                      +++ apply ctx_id_right_is_id.
+                      +++ eapply alpha_sym. constructor. eauto with α_eq_db.
+           ++ constructor. apply legalRenSwap_id.
         -- change (ctx_id_right ren) with (nil ++ ctx_id_right ren).
            apply alpha_extend_ids_right.
            ++ apply ctx_id_right_is_id.
@@ -183,37 +410,36 @@ Proof.
     exists (tmlam y A tα); split.
     + apply step_abs_d. assumption.
     + apply alpha_lam; assumption.    
-Admitted.
+Qed.
 
 Lemma step_d_implies_step_gu_na t t' : 
     step_d t t' ->  
     {t_α & step_gu_naive t t_α * (nil ⊢ t' ~ t_α)}.
 Proof.
-    remember (to_unique_binders t) as t_GU.
+    remember (to_GU t) as t_GU.
     assert (nil ⊢ t ~ t_GU) as H_alpha.
     {
       subst.
-      apply to_unique_binders_alpha.
+      apply to_GU__alpha.
     }
-    assert (GU_vars t_GU) as H_GU.
+    assert (GU t_GU) as H_GU.
     {
       subst.
-      apply to_unique_binders_unique.
+      apply to_GU__GU.
     }
     intros.
     remember (step_d_preserves_alpha H_alpha H) as Hstep_GU.
     destruct Hstep_GU as [t_GU' [Hstep_GU Halpha_GU] ].
     exists t_GU'.
-    split.
-    - clear HeqHstep_GU.
-        apply GU_step_d_implies_step_na in Hstep_GU.
-        + subst. constructor. auto.
-        + auto.
-    - auto. 
+    split; auto.
+    clear HeqHstep_GU.
+    apply GU_step_d_implies_step_na in Hstep_GU.
+    + apply step_gu_naive_intro with (s' := t_GU); auto.
+    + subst. auto.
 Qed.
 
 Theorem α_preserves_sn_d s s' :
-  Alpha [] s s' -> (@sn step_d) s -> (@sn step_d) s'.
+  Alpha [] s s' -> (@sn term step_d) s -> (@sn term step_d) s'.
 Proof.
   intros Hα Hsn.
   generalize dependent s'.
@@ -226,12 +452,12 @@ Proof.
     - eapply alpha_sym in Hα. exact Hα. apply alpha_sym_nil.
     - assumption.
   }
-  eapply H.
+  eapply X.
   - exact Hstep'.
   - eapply alpha_sym. apply alpha_sym_nil. exact Hα'.
 Qed.
 
-Lemma SN_na_to_SN_d t : (@sn step_gu_naive) t -> (@sn step_d) t.
+Lemma SN_na_to_SN_d t : (@sn term step_gu_naive) t -> (@sn term step_d) t.
 Proof.
   intros Hsn_nd.
   apply SNI.
@@ -243,10 +469,17 @@ Proof.
     eapply step_d_implies_step_gu_na; eauto.
   }
   destruct Hstep_alpha as [t' [Hstep Halpha] ].
-  specialize (H t' Hstep).
+  specialize (X t' Hstep).
   apply α_preserves_sn_d with t'.
   - eapply alpha_sym; [apply alpha_sym_nil |].
     assumption.
   - apply SNI. 
-    exact H.
-Qed. *)
+    exact X.
+Qed.
+
+Theorem strong_normalization E s T : has_type E s T -> (@sn term step_d) s.
+  intros.
+  apply SN_naive in H. 
+  apply SN_na_to_SN_d.
+  assumption.
+Qed.
