src/PlutusIR/Semantics/Static/normaliser_STLC/gu_naive/port_plut2.v
@@ -1,0 +1,373 @@
+
+From Equations Require Import Equations.
+Require Import Coq.Lists.List.
+Local Open Scope list_scope.
+
+Require Import Lia.
+
+Require Import Coq.Program.Basics.
+Require Import Coq.Strings.String.
+Local Open Scope string_scope.
+Require Import Coq.Arith.PeanoNat.
+Import ListNotations.
+Require Import Ascii.
+
+From PlutusCert Require Import port_plut util Util.List. (* I don't understand why we need this for ftv defintion*)
+
+Inductive BType := L | F. (* Lam or Forall*)
+
+(** Types *)
+Inductive term :=
+  | tmvar : string -> term
+  | tmlam : BType -> string -> type -> term -> term
+  | tmapp : term -> term -> term
+.
+
+(** Substitutions *)
+Function ftv (T : term) : list string :=
+    match T with
+    | tmvar X =>
+        [X]
+    | tmlam B X K1 T' =>
+        remove string_dec X (ftv T')
+    | tmapp T1 T2 =>
+        ftv T1 ++ ftv T2
+    end.
+
+Fixpoint btv (T : term) : list string :=
+    match T with
+    | tmvar X =>
+        []
+    | tmlam B X K1 T' =>
+      X :: btv T'
+    | tmapp T1 T2 =>
+        btv T1 ++ btv T2
+    end.
+
+(* Bound and free type variables *)
+Fixpoint tv (s : term) : list string :=
+  match s with
+  | tmvar x => x::nil
+  | tmlam B x A s => x :: tv s
+  | tmapp s t => tv s ++ tv t
+  end.
+
+(** * Capture-avoiding substitution of types *)
+
+Fixpoint tv_keys_env (sigma : list (string * term)) : list string :=
+  match sigma with
+  | nil => nil
+  | (x, t)::sigma' => x :: (tv t) ++ (tv_keys_env sigma')
+  end.
+
+Definition fresh2 (sigma : list (string * term)) (T : term) : string :=
+  "a" (* new*)
+  ++ String.concat EmptyString (
+    tv_keys_env sigma ++ tv T
+  ).
+
+Definition fresh (X : string) (U T : term) : string :=
+  "a" ++ X ++ (String.concat EmptyString (ftv U)) ++ (String.concat EmptyString (ftv T)).
+
+Lemma fresh__X : forall X U T,
+    X <> fresh X U T.
+Proof with eauto.
+  intros. intros Hcon.
+  induction X; induction (ftv U); induction (ftv T).
+  all: simpl in Hcon.
+  all: inversion Hcon; subst...
+Qed.
+
+Lemma fresh__S : forall X U T,
+    ~ In (fresh X U T) (ftv U).
+Proof. Abort.
+
+Lemma fresh__T : forall X U T,
+    ~ In (fresh X U T) (ftv T).
+Proof. Abort.
+
+Fixpoint rename (X Y : string) (T : term) :=
+  match T with
+  | tmvar Z =>
+      if X =? Z then tmvar Y else tmvar Z
+  | tmlam B Z K T0 =>
+      if X =? Z then tmlam B Z K T0
+      else tmlam B Z K (rename X Y T0)
+  | tmapp T1 T2 =>
+      tmapp (rename X Y T1) (rename X Y T2)
+  end.
+
+(* Size of a term *)
+
+Fixpoint size (T : term) : nat :=
+  match T with
+  | tmvar Y => 1
+  | tmlam B bX K T0 => 1 + size T0
+  | tmapp T1 T2 => 1 + size T1 + size T2
+  end.
+
+
+Lemma rename_preserves_size : forall T X Y,
+    size T = size (rename X Y T).
+Proof.
+  unfold rename.
+  induction T; intros; simpl; eauto.
+  - destruct (X =? s); eauto.
+  - destruct (X =? s); simpl; eauto.
+Qed.
+
+Equations? substituteTCA (X : string) (U T : term) : term by wf (size T) :=
+  substituteTCA X U (tmvar Y) =>
+      if X =? Y then U else tmvar Y ;
+  substituteTCA X U (@tmlam B Y K T) =>
+      if X =? Y
+        then
+          @tmlam B Y K T
+        else
+          if existsb (String.eqb Y) (ftv U)
+            then
+              let Y' := fresh2 ((Y, tmvar Y)::(X, U)::nil) T in
+              let T' := rename Y Y' T in
+              @tmlam B Y' K (substituteTCA X U T')
+            else
+              @tmlam B Y K (substituteTCA X U T) ;
+  substituteTCA X U (tmapp T1 T2) =>
+      tmapp (substituteTCA X U T1) (substituteTCA X U T2)
+  .
+Proof.
+  all: try solve
+    [ lia
+    || replace T' with (rename Y Y' T); eauto; rewrite <- rename_preserves_size; eauto
+    ].
+Qed.
+
+
+Inductive step_nd : term -> term -> Type :=
+| step_beta_d (B : BType) (x : string) (A : type) (s t : term) :
+  (* This allows for more steps then should be allowed.
+      e.g. tmapp (forall B x A s) t) will now beta reduce.
+
+      But that is no problem! As long as step_nd allows all steps that step_plut allows.
+  *)
+    step_nd (tmapp (@tmlam B x A s) t) (substituteTCA x t s) (* capture avoiding conservative substitutions *)
+| step_appL_d s1 s2 t :
+    step_nd s1 s2 -> step_nd (tmapp s1 t) (tmapp s2 t)
+| step_appR_d s t1 t2 :
+    step_nd t1 t2 -> step_nd (tmapp s t1) (tmapp s t2)
+| step_abs_d B x A s1 s2 :
+    step_nd s1 s2 -> step_nd (@tmlam B x A s1) (@tmlam B x A s2).
+
+Set Implicit Arguments.
+
+(** Substitutions *)
+
+(* from plut to annotated stlc*)
+Fixpoint f (t : term_plut) : term :=
+  match t with
+  | plutvar x => tmvar x
+  | plutlam x A t => @tmlam L x A (f t)
+  | plutforall x A t => @tmlam F x A (f t)
+  | plutapp t1 t2 => tmapp (f t1) (f t2)
+  end.
+
+Require Import Coq.Program.Equality.
+
+Lemma f_preserves_rename s fr T :
+  rename s fr (f T) = f (port_plut.rename s fr T).
+Proof.
+  induction T.
+  - simpl.
+    destr_eqb_eq s s0.
+    + simpl. auto.
+    + simpl. auto.
+  - simpl.
+    destr_eqb_eq s s0.
+    + simpl. auto.
+    + simpl. f_equal. auto.
+  - simpl.
+    destr_eqb_eq s s0.
+    + simpl. auto.
+    + simpl. f_equal; auto.
+  - simpl.
+    f_equal; auto.
+Qed.
+
+Lemma f_preserves_ftv T :
+  ftv (f T) = port_plut.ftv T.
+Proof.
+  induction T; simpl; try f_equal; auto.
+Qed.
+
+Lemma f_preserves_tv T :
+  tv (f T) = port_plut.tv T.
+Proof.
+  induction T; simpl; try f_equal; auto.
+Qed.
+
+Lemma f_preserves_fresh2 x y s s' T :
+  fresh2 ((x, f s)::(y, f s')::nil) (f T) = port_plut.fresh2 ((x, s)::(y, s')::nil) T.
+Proof.
+  simpl.
+  unfold fresh2.
+  unfold port_plut.fresh2.
+  rewrite f_preserves_tv.
+  assert (Htv_keys_env: (tv_keys_env
+  [(x, f s); (y, f s')] = port_plut.tv_keys_env [(x, s); (y, s')])).
+  {
+    unfold tv_keys_env.
+    unfold port_plut.tv_keys_env.
+    f_equal.
+    rewrite f_preserves_tv.
+    f_equal.
+    rewrite f_preserves_tv.
+    f_equal.
+  }
+  rewrite Htv_keys_env.
+  reflexivity.
+Qed.
+
+Require Import Coq.Arith.Wf_nat.
+
+Lemma f_preserves_substituteTCA X U T :
+  (f (port_plut.substituteTCA X U T)) = (substituteTCA X (f U) (f T)).
+Proof.
+  remember (f T) as fT.
+  remember (size fT) as n.
+  generalize dependent fT.
+  generalize dependent T.
+  induction n using lt_wf_ind.
+  intros.
+  dependent induction fT; subst.
+  + induction T; subst; inversion HeqfT; subst.
+    autorewrite with substituteTCA.
+    destr_eqb_eq X s0; auto.
+  + induction T; subst; inversion HeqfT; subst.
+    * autorewrite with substituteTCA.
+      destr_eqb_eq X s0; eauto.
+      rewrite <- (f_preserves_ftv).
+      destruct (existsb (String.eqb s0) (ftv (f U))) eqn:Heq.
+      -- 
+          simpl.
+          remember (fresh2 _ _) as fr.
+          remember (port_plut.fresh2 _ _) as fr'.
+          assert (Hfr_pres: fr' = fr).
+          {
+            subst.
+            symmetry.
+            assert (Hfpluvar: f (plutvar s0) = tmvar s0) by auto.
+            rewrite <- Hfpluvar.
+            rewrite f_preserves_fresh2.
+            reflexivity.
+          }
+          rewrite Hfr_pres.
+          f_equal.
+          ++ eapply H; eauto.
+            ** rewrite <- rename_preserves_size.
+               simpl.
+               lia.
+            ** apply f_preserves_rename.
+      -- simpl.
+          f_equal.
+          eapply H; eauto. simpl. lia.
+
+
+
+      (* TODO: EXACTLY IDENTICAL TO ABOVE*)
+      * autorewrite with substituteTCA.
+      destr_eqb_eq X s0; eauto.
+      rewrite <- (f_preserves_ftv).
+      destruct (existsb (String.eqb s0) (ftv (f U))) eqn:Heq.
+      -- 
+          simpl.
+          remember (fresh2 _ _) as fr.
+          remember (port_plut.fresh2 _ _) as fr'.
+          assert (Hfr_pres: fr' = fr).
+          {
+            subst.
+            symmetry.
+            assert (Hfpluvar: f (plutvar s0) = tmvar s0) by auto.
+            rewrite <- Hfpluvar.
+            rewrite f_preserves_fresh2.
+            reflexivity.
+          }
+          rewrite Hfr_pres.
+          f_equal.
+          ++ eapply H; eauto.
+            ** rewrite <- rename_preserves_size.
+               simpl.
+               lia.
+            ** apply f_preserves_rename.
+      -- simpl.
+          f_equal.
+          eapply H; eauto. simpl. lia.
+
+        (* END TODO*)
+
+  + induction T; subst; inversion HeqfT; subst.
+    
+    autorewrite with substituteTCA.
+    simpl.
+    f_equal; eauto.
+    * eapply H; auto. simpl. lia.
+    * eapply H; auto. simpl. lia.
+Qed.
+
+        
+Theorem f_preserves_step s s' :
+  step_plut s s' -> step_nd (f s) (f s').
+Proof.
+  intros H.
+  induction H; simpl; eauto.
+  - rewrite f_preserves_substituteTCA.
+    constructor.
+  - constructor. assumption.
+  - constructor. assumption.
+  - constructor. assumption.
+  - constructor. assumption.
+Qed.
+
+Inductive sn {X : Type} {e : X -> X -> Type } x : Type :=
+| SNI : (forall y, e x y -> sn y) -> sn x.
+
+Lemma sn_preimage2 {e2 : term_plut -> term_plut -> Type} {e : term -> term -> Type} (h : term_plut -> term) (x : term_plut) :
+  (forall x y, e2 x y -> e (h x) (h y)) -> @sn term e (h x) -> @sn term_plut e2 x.
+Proof.
+  intros A B.
+  remember (h x) as v. (* this allows us to keep B : sn v as an hypothesis*)
+  generalize dependent h.
+  generalize dependent x.
+  induction B.
+  intros x0 h A eqn.
+  apply SNI.
+  intros y C.
+  apply A in C.
+  
+  specialize (X (h y)).
+  rewrite <- eqn in C.
+  eapply X.
+  - assumption.
+  - exact A.
+  - reflexivity.
+Qed.
+
+(* todo: well kinded assumption.
+  So we need to convert that from the step_plut one.
+  if s is plut_well_kinded, then (f s) is nd_well_kinded
+ *)
+Theorem sn_step_nd : forall s, @sn term step_nd s.
+Admitted.
+
+Theorem sn_step_plut : forall s, @sn term step_nd (f s) -> @sn term_plut step_plut s.
+Proof.
+  intros s.
+  eapply @sn_preimage2 with (h := f) (e2 := step_plut) (e := step_nd).
+  apply f_preserves_step.
+Qed.
+
+Corollary sn_step_plut2 : forall s, @sn term_plut step_plut s.
+Proof.
+  intros s.
+  eapply sn_preimage2 with (h := f).
+  apply f_preserves_step.
+  apply sn_step_nd.
+Qed.
